src/named/Subst.v
@@ -83,9 +83,9 @@ Fixpoint cat_lang_sub_r c e G_l : exp :=
   | _ => {{e #"ERR"}}
   end.
   
-#[refine]
 Instance rec_cat_lang : LangRecognize cat_lang :=
-  { le_sort_dec _ _ t1 t2 := t1 == t2;
+  { le_sort_dec := generic_sort_dec_fuel 10 cat_lang;
+    decide_le_sort := @generic_decide_le_sort 10 cat_lang;
     term_args_elab c s name t := 
       match name, t, s with
       | "id", scon "sub" [:: _; G],_ => [:: G]
@@ -96,33 +96,12 @@ Instance rec_cat_lang : LangRecognize cat_lang :=
       end%string;
     sort_args_elab c s _ := s
   }.
-Proof.
-  {
-    intros n c t1 t2 _ _ _.
-    ltac1:(move /eqP ->).
-    apply le_sort_refl.
-  }
-Defined.
 
 Lemma cat_lang_wf : wf_lang cat_lang.
 Proof.
   apply (@decide_wf_lang _ _ 100).
   vm_compute; reflexivity.
 Qed.
-
-Derive elab_cat_lang
-       SuchThat (elab_lang cat_lang elab_cat_lang)
-       As elab_cat_lang_pf.
-Proof.
-  repeat (elab (fun () => reflexivity)).
-Qed. 
-
-Instance elab_cat_lang_inst : Elaborated cat_lang :=
-  {
-  elaboration := elab_cat_lang;
-  elab_pf := elab_cat_lang_pf;
-  }.
-
 
 Definition subst_lang' : lang :=
  [::[:> 
@@ -145,8 +124,8 @@ Definition subst_lang' : lang :=
        "f" : #"sub" %"G1" %"G2", "g" : #"sub" %"G2" %"G3",
        "A" : #"ty" %"G3", "e" : #"el" %"G3" %"A"
        ----------------------------------------------- ("el_subst_cmp")
-       #"el_subst" (#"cmp" %"f" %"g") %"e"
-       = #"el_subst" %"f" (#"el_subst" %"g" %"e")
+       #"el_subst" %"f" (#"el_subst" %"g" %"e")
+       = #"el_subst" (#"cmp" %"f" %"g") %"e"
        : #"el" %"G1" (#"ty_subst" (#"cmp" %"f" %"g") %"A")
   ]; 
   [:> "G" : #"env", "A" : #"ty" %"G", "e" : #"el" %"G" %"A"
@@ -157,8 +136,8 @@ Definition subst_lang' : lang :=
        "f" : #"sub" %"G1" %"G2", "g" : #"sub" %"G2" %"G3",
        "A" : #"ty" %"G3"
        ----------------------------------------------- ("ty_subst_cmp")
-       #"ty_subst" (#"cmp" %"f" %"g") %"A"
-       = #"ty_subst" %"f" (#"ty_subst" %"g" %"A")
+       #"ty_subst" %"f" (#"ty_subst" %"g" %"A")
+       = #"ty_subst" (#"cmp" %"f" %"g") %"A"
        : #"ty" %"G1"
   ];              
   [:> "G" : #"env", "A" : #"ty" %"G"
@@ -183,7 +162,301 @@ Definition subst_lang' : lang :=
   [s| "G" : #"env" 
       -----------------------------------------------
       #"ty" "G" srt
-  ]]%irule++cat_lang.
+  ]]%arule++cat_lang.
+
+
+(* combines le_sort_by and le_sort_subst *)
+Lemma le_sort_by' name l c : forall c' e1 e2 s1 s2 e1' e2',
+    [s> !c' 
+         ----------------------------------------------- (name)
+         {e1} = {e2} ]%arule \in l ->
+    len_eq s1 c' ->
+    len_eq s2 c' -> 
+    e1' = e1[/with_names_from c' s1/] ->
+    e2' = e2[/with_names_from c' s2/] ->
+    le_subst l c c' (with_names_from c' s1) (with_names_from c' s2) ->
+    le_sort l c e1' e2'.
+Proof using .
+  intros.
+  rewrite H2; clear H2.
+  rewrite H3; clear H3.
+  eapply le_sort_subst>[| eapply le_sort_by; eauto].
+  auto.
+Qed.
+
+(* combines le_term_by and le_term_subst *)
+Lemma le_term_by' name l c : forall c' t e1 e2 s1 s2 t' e1' e2',
+    [:> !c' 
+        ----------------------------------------------- (name)
+        {e1} = {e2} : {t}]%arule \in l ->
+    len_eq s1 c' ->
+    len_eq s2 c' ->                          
+    t' = t[/with_names_from c' s2/] ->
+    e1' = e1[/with_names_from c' s1/] ->
+    e2' = e2[/with_names_from c' s2/] ->
+      le_subst l c c' (with_names_from c' s1) (with_names_from c' s2) ->
+    le_term l c t' e1' e2'.
+Proof using .
+  intros.
+  rewrite H2; clear H2.
+  rewrite H3; clear H3.
+  rewrite H4; clear H4.
+  eapply le_term_subst>[| eapply le_term_by; eauto].
+  auto.
+Qed.
+(*
+
+(*TODO: temp; needs improvement*)
+Lemma le_sort_refl' name l c args : forall c' s1 s2 e1' e2',
+    (name, sort_rule c' args) \in l ->
+    len_eq s1 c' ->
+    len_eq s2 c' ->
+    len_eq s1 args ->
+    e1' = scon name s1 ->
+    e2' = scon name s2 ->
+    le_subst l c c' (with_names_from c' s1) (with_names_from c' s2) ->
+    le_sort l c e1' e2'.
+Proof using .
+Admitted.
+  
+
+Lemma nth_tail_in_bound {A : eqType} (e:A) m n l
+        : m <= n -> e \in nth_tail n l -> e \in nth_tail m l.
+Admitted.
+ *)
+
+Fixpoint sub_decompose g f : exp :=
+  if f == g then {{e #"id"}}
+  else match f with
+       | con "cmp" [:: h; f'] =>
+         {{e #"cmp" {sub_decompose g f'} {h} }}
+       | _ => {{e #"ERR"}}
+       end.
+
+(* TODO: the right way to do the elab is some bidirectional thing 
+   I think. For now special casing el_subst
+*)         
+Instance rec_subst_lang' : LangRecognize subst_lang' :=
+  {  le_sort_dec := generic_sort_dec_fuel 10 subst_lang';
+    decide_le_sort := @generic_decide_le_sort 10 subst_lang';
+(*  le_sort_dec n c t1 t2 :=
+      (t1 == t2) ||
+      ((n <= 6) &&
+       (c == [:: ("e"%string, {{s#"el" %"G3" %"A"}}); ("A"%string, {{s#"ty" %"G3"}});
+        ("g"%string, {{s#"sub" %"G2" %"G3"}}); ("f"%string, {{s#"sub" %"G1" %"G2"}}); 
+       ("G3"%string, {{s#"env"}}); ("G2"%string, {{s#"env"}}); ("G1"%string, {{s#"env"}})])&&
+       (t1=={{s#"el" %"G1" (#"ty_subst" %"f" (#"ty_subst" %"g" %"A"))}})&&
+       (t2=={{s#"el" %"G1" (#"ty_subst" (#"cmp" %"f" %"g") %"A")}}));*)
+    term_args_elab c s name t := 
+      match name, t, s with
+      | "forget", scon "sub" [:: _; G],_ => [:: G]
+      | "id", scon "sub" [:: _; G],_ => [:: G]
+      | "cmp", scon "sub" [:: G3; G1], [:: g; f] =>
+        let G2 := cat_lang_sub_r c f G1 in
+        [:: g; f; G3; G2; G1]
+      | "ty_subst", scon "ty" [:: G], [:: A; g] =>
+        let G' := cat_lang_sub_r c g G in
+        [:: A; g; G'; G]
+      | "el_subst", scon "el" [:: (con "ty_subst" [:: A; f]); G], [:: e; g] =>
+        let G' := cat_lang_sub_r c g G in
+        (* need to pull a g substitution off of f;
+           first run f to simplify
+         *)
+        let f' := term_par_step_n subst_lang' f 100 in
+        let f'' := sub_decompose g f' in
+        [:: e; (con "ty_subst" [:: A; f'']); g; G'; G]
+      (* special case for id subst since it can disappear; only works if g ~ id*)
+      | "el_subst", scon "el" [:: A; G], [:: e; g] =>
+        let G' := cat_lang_sub_r c g G in
+        (* need to pull a g substitution off of f;
+           first run f to simplify
+         *)
+        [:: e; A; g; G'; G]
+      | _,_,_ => s
+      end%string;
+    sort_args_elab c s _ := s
+  }.
+(*
+Proof.
+  {
+    intros n c t1 t2 _ _ _.
+    ltac1:(move /orP => []).
+    {
+      ltac1:(move /eqP ->);
+        apply le_sort_refl.
+    }
+    {
+      ltac1:(move => /andP [] /andP [] /andP [nlt] /eqP -> /eqP -> /eqP ->).
+      eapply (le_sort_refl' (name:="el"%string)).
+      ltac1:(simple eapply nth_tail_in_bound); eauto.
+      match!goal with
+      | [|- is_true((?n,?e)\in ?l)]=>
+        (*TODO: this can be improved a bit*)
+        assert ($e = named_list_lookup $e $l $n); cbv; solve[auto]
+      end.
+      repeat constructor.
+      repeat constructor.
+      repeat constructor.
+      reflexivity.
+      reflexivity.
+      {
+        constructor.
+        constructor.
+        constructor.
+        {
+          simpl.
+          apply le_term_refl.
+        }
+        {
+          eapply (le_term_by' (name:="ty_subst_cmp"%string)); eauto.
+          
+          ltac1:(simple eapply nth_tail_in_bound); eauto.
+          match!goal with
+          | [|- is_true((?n,?e)\in ?l)]=>
+            (*TODO: this can be improved a bit*)
+            assert ($e = named_list_lookup $e $l $n); cbv; solve[auto]
+          end.
+          repeat constructor.
+          repeat constructor.
+          reflexivity.
+          reflexivity.
+          reflexivity.
+          simpl.
+          repeat (constructor>[| eapply le_term_refl]).
+          constructor.
+        }
+      }
+    }
+  }
+  Unshelve.
+  exact ({{e%"ERR"}}).
+  exact ({{e%"ERR"}}).
+Defined.
+*)
+    
+Lemma unfold_wf_term_dec l lr n c name s t fuel'
+  : wf_term_dec lr  n c (con name s) t (S fuel')
+    = match named_list_lookup_err (nth_tail n l) name with
+      | Some (term_rule c' args t') =>
+        let es := @term_args_elab l lr c s name t in
+        (wf_sort_dec lr n c t'[/with_names_from c' es/] fuel') &&
+        (le_sort_dec n c t'[/with_names_from c' es/] t) &&
+        (wf_args_dec lr n c s args es c' fuel')
+      | _ => false
+      end.
+Proof.
+  reflexivity.
+Qed.
+
+Lemma unfold_wf_args_dec l (lr : LangRecognize l) n c s args es c' fuel'
+  : wf_args_dec lr n c s args es c' (S fuel') =
+         match c',es, args, s with
+         | [::], [::], [::], [::] => true
+         | [::], _, _, _ => false
+         | (name,t)::c'', [::], _, _ => false
+         | (name,t)::c'', e::es', [::], [::] =>
+           (wf_term_dec lr n c e t[/with_names_from c'' es'/] fuel') &&
+           (wf_args_dec lr n c [::] [::] es' c'' fuel')
+         | (name,t)::c'', e::es', name'::args', e'::s' =>
+           if name == name'
+           then (e == e') &&
+                (wf_term_dec lr n c e t[/with_names_from c'' es'/] fuel') &&
+                (wf_args_dec lr n c s' args' es' c'' fuel')
+           else (wf_term_dec lr n c e t[/with_names_from c'' es'/] fuel') &&
+                (wf_args_dec lr n c s args es' c'' fuel')
+         | _,_,_,_ => false (*TODO?*)
+         end.
+Proof.
+  reflexivity.
+Qed.
+
+Lemma subst_lang'_wf : wf_lang subst_lang'.
+Proof.
+  apply (@decide_wf_lang _ _ 100); vm_compute; reflexivity.
+Qed.
+
+
+(*
+Fixpoint subst_lang'_reduce_sub e : exp :=
+  match e with
+  | con "cmp" [::g; f] =>
+    match subst_lang'_reduce_sub g, subst_lang'_reduce_sub f with
+    | con "id" [::], f' => f'
+    | g', con "id" [::] => g'
+    | g',f' => (*TODO: incomplete; cmp assoc*) {{e #"cmp" {f'} {g'} }}
+    end
+  (* TODO: incomplete*)
+  | _ => e
+  end.
+
+Fixpoint subst_lang'_reduce_ty e : exp :=
+  match e with
+  | con "ty_subst" [:: A; g] =>
+    match subst_lang'_reduce_sub g, subst_lang'_reduce_ty A with
+    | con "id" [::], A' => A'
+    | g', con "ty_subst" [:: B; f] =>
+      let gf := subst_lang'_reduce_sub {{e #"cmp" {g} {f} }} in
+      {{e #"ty_subst" {gf} {B} }}
+    | g', A' => {{e #"ty_subst" {g'} {A'} }}
+    end
+  (* TODO: incomplete*)
+  | _ => e
+  end.
+*)
+(* TODO: congruence is trickier for this version*)
+(*
+Lemma subst_lang'_reduce_sub_le c e t
+  : wf_term subst_lang' c e t ->
+    le_term subst_lang' c t e (subst_lang'_reduce_sub e).
+Proof.
+  induction e.
+  { intros _; simpl; eapply le_term_refl. }
+  {
+    ltac1:(case neq: (n == "cmp")%string).
+    {
+      ltac1:(move: neq => /eqP ->).
+      repeat (destruct l;
+              try (solve[intros; simpl; eapply le_term_refl])).
+      destruct H.
+      destruct H0.
+      destruct H1.
+      Search _ le_term.
+      apply Tactics.le_term_refl'.
+      
+    }
+    {
+      simpl.
+      destruct l; simpl.
+      { intros; simpl; eapply le_term_refl. }
+*)
+(*
+  
+#[refine]
+Instance rec_subst_lang' : LangRecognize subst_lang' :=
+  { le_sort_dec _ _ t1 t2 :=
+      match t1,t2 with
+      | scon "ty" [::A1; G1], scon "ty" [::A2; G2] =>
+        (G1 == G2)&&(subst_lang'_reduce_ty A1 == subst_lang'_reduce_ty A2)
+      | _, _ => t1 == t2
+      end;
+      (* TODO: extend *)
+    term_args_elab c s name t := 
+      match name, t, s with
+      | "id", scon "sub" [:: _; G],_ => [:: G]
+      | "cmp", scon "sub" [:: G3; G1], [:: g; f] =>
+        let G2 := cat_lang_sub_r c f G1 in
+        [:: g; f; G3; G2; G1]
+      | _,_,_ => s
+      end%string;
+    sort_args_elab c s _ := s
+  }.
+Proof.
+  {
+    intros n c t1 t2 _ _ _.
+    ltac1:(move /eqP ->).
+    apply le_sort_refl.
+  }
+Defined.
 
 Derive elab_subst_lang'
        SuchThat (elab_lang subst_lang' elab_subst_lang')
@@ -206,7 +479,7 @@ Instance elab_subst_lang'_inst : Elaborated subst_lang' :=
   elaboration := elab_subst_lang';
   elab_pf := elab_subst_lang'_pf;
   }.
-
+*)
 
 (****************************
  Nth-tail section; TODO: is any of this needed?
@@ -227,32 +500,7 @@ Arguments is_fst {A} !l/.
 
 (*Temporary, just for the following lemma:*)
 Arguments nth_tail {A} !n l/.
-Lemma elab_lang_cons'_helper
-  : forall (l : named_list rule) (el : ARule.lang) (name : string) 
-           (r : rule) (er : ARule.rule),
-    fresh name l ->
-    (* TODO: is_fst for lang?; need eqtype for IExp; just get rid of iexp?*)
-    is_fst el (name,er) ->
-    elab_lang l (nth_tail 1 el) ->
-    elab_rule (nth_tail 1 el) r er ->
-    elab_lang ((name,r)::l) el.
-Proof.
-  intros l el.
-  revert l.
-  destruct el.
-  {
-    intros.
-    vm_compute in H0.
-    inversion H0.
-  }
-  {
-    intros.
-    simpl in H0,H1,H2.
-    ltac1:(move: H0 => /eqP H0).
-    subst.
-    constructor; auto.
-  }
-Qed.
+
 
 Lemma nth_tail_S_cons {A} n (e:A) l : nth_tail n.+1 (e::l) = nth_tail n l.
 Proof.
@@ -271,19 +519,6 @@ Proof.
     }
   }
 Qed.    
-
-Lemma elab_lang_cons' n l el name r er
-  : fresh name l ->
-    (* TODO: is_fst for lang?; need eqtype for IExp; just get rid of iexp?*)
-    is_fst (nth_tail n el) (name,er) ->
-    elab_lang l (nth_tail n.+1 el) ->
-    elab_rule (nth_tail n.+1 el) r er ->
-    elab_lang ((name,r)::l) (nth_tail n el).
-Proof.
-  intros.
-  eapply (@elab_lang_cons'_helper l (nth_tail n el));
-    rewrite ?nth_tail_add1; eauto.
-Qed.
 
 
 Arguments nth_tail : simpl never.
@@ -339,139 +574,8 @@ Definition subst_lang : lang :=
   [:| "G" : #"env", "A": #"ty" %"G"
        -----------------------------------------------
        #"ext" "G" "A" : #"env"
-  ]]%irule++subst_lang'.
+  ]]%arule++subst_lang'.
 
-Derive elab_subst_lang
-       SuchThat (elab_lang subst_lang elab_subst_lang)
-       As elab_subst_lang_pf.
-Proof.
-  repeat (elab(fun()=>
-       lazy_match! goal with
-       | [|-Core.le_sort _ _ (Exp.scon ?name _) _] => eapply (@Core.le_sort_refl' $name)
-       | [|-Core.le_sort _ _ _ (Exp.scon ?name _)] => eapply (@Core.le_sort_refl' $name)
-       | [|-Core.le_term _ _ _ _ (Exp.var _)] => reflexivity
-       | [|-Core.le_term _ _ _ (Exp.var _) _] => reflexivity
-       | [|-Core.le_term _ _ _ (Exp.con "ext" _) _] => eapply (@Core.le_term_refl' "ext"%string)
-       | [|-Core.le_term _ _ _ _ (Exp.con "ext" _)] => eapply (@Core.le_term_refl' "ext"%string)
-       | [|-Core.le_term _ _ _
-                         (Exp.con "ty_subst" [:: _; ?g; ?gg'; ?gg])
-                         (Exp.con "ty_subst" [:: _; ?g; ?gg'; ?gg])] =>
-          eapply (@Core.le_term_refl' "ty_subst"%string)
-               end)).
-  (*TODO: why is this not done already?*)
-  Focus 3.
-  reflexivity.
-  
-  elab(fun()=>()).
-  elab(fun()=>()).
-  elab(fun()=>()).
-  elab(fun()=>()).
-  elab(fun()=>()).
-  elab(fun()=>()).
-  elab(fun()=>()).
-
-  Focus 2.
-  elab(fun()=>()).
-
-  Focus 5.
-  reflexivity.
-  elab(fun()=>()).
-  elab(fun()=>()).
-  elab(fun()=>()).
-  elab(fun()=>()).
-  elab(fun()=>()).
-  elab(fun()=>()).
-  elab(fun()=>()).
-  elab(fun()=>()).
-  elab(fun()=>()).
-  elab(fun()=>()).
-  elab(fun()=>()).
-  elab(fun()=>()).
-  elab(fun()=>()).
-  elab(fun()=>()).
-  elab(fun()=>()).
-  elab(fun()=>()).
-  elab(fun()=>()).
-
-  Focus 2.
-  elab(fun()=>()).
-
-  Focus 5.
-  reflexivity.
-  elab(fun()=>()).
-  elab(fun()=>()).
-  elab(fun()=>()).
-  elab(fun()=>()).
-  simpl.
-
-  reflexivity.
-  elab(fun()=>()).
-  elab(fun()=>()).
-  elab(fun()=>()).
-  elab(fun()=>()).
-  elab(fun()=>()).
-  elab(fun()=>()).
-  elab(fun()=>()).
-  elab(fun()=>()).
-  {
-    eapply Core.le_term_trans.
-    symmetry.
-    eapply (@Core.le_term_by' "ty_subst_cmp"%string);elab(fun()=>reflexivity).
-    eapply (Core.le_term_refl');elab(fun()=>easy_le_tac()).
-  }
-  
-  elab(fun()=>()).
-  elab(fun()=>()).
-  elab(fun()=>()).
-  elab(fun()=>()).
-  elab(fun()=>()).
-  elab(fun()=>()).
-  elab(fun()=>()).
-  elab(fun()=>()).
-  elab(fun()=>()).
-  elab(fun()=>()).
-  elab(fun()=>()).
-  elab(fun()=>()).
-  elab(fun()=>()).
-
-  reflexivity.
-  elab(fun()=>()).
-  elab(fun()=>()).
-  elab(fun()=>()).
-  elab(fun()=>()).
-
-  symmetry.
-  eapply (@Core.le_term_by' "ty_subst_cmp"%string);elab(fun()=>reflexivity).
-  elab(fun()=>()).
-  elab(fun()=>()).
-  elab(fun()=>()).
-  elab(fun()=>()).
-  elab(fun()=>()).
-  elab(fun()=>()).
-  elab(fun()=>()).
-  elab(fun()=>()).
-  elab(fun()=>()).
-  elab(fun()=>()).
-  elab(fun()=>()).
-  elab(fun()=>()).
-  elab(fun()=>()).
-  elab(fun()=>()).
-  elab(fun()=>()).
-  elab(fun()=>()).
-  elab(fun()=>()).
-  elab(fun()=>()).
-  elab(fun()=>()).
-  elab(fun()=>()).
-  elab(fun()=>()).
-  elab(fun()=>()).
-  elab(fun()=>()).
-  elab(fun()=>()).
-Qed.
-
- 
-    
-Instance elab_subst_lang_inst : Elaborated subst_lang :=
-  {
-  elaboration := elab_subst_lang;
-  elab_pf := elab_subst_lang_pf;
-  }.
+Eval compute in (term_par_step_n subst_lang
+                               {{e #"el_subst" (#"snoc" (#"snoc" (#"snoc" #"forget" %"y") %"x") %"e")
+                                   (#"el_subst" #"wkn" (#"el_subst" #"wkn" #"hd"))}} 7).
